proofs/fstar/extraction-lax/Bertie.Server.fsti
@@ -1,0 +1,29 @@
+module Bertie.Server
+#set-options "--fuel 0 --ifuel 1 --z3rlimit 15"
+open Core
+open FStar.Mul
+
+type t_ServerDB = {
+  f_server_name:Bertie.Tls13utils.t_Bytes;
+  f_cert:Bertie.Tls13utils.t_Bytes;
+  f_sk:Bertie.Tls13utils.t_Bytes;
+  f_psk_opt:Core.Option.t_Option (Bertie.Tls13utils.t_Bytes & Bertie.Tls13utils.t_Bytes)
+}
+
+val impl__ServerDB__new
+      (server_name cert sk: Bertie.Tls13utils.t_Bytes)
+      (psk_opt: Core.Option.t_Option (Bertie.Tls13utils.t_Bytes & Bertie.Tls13utils.t_Bytes))
+    : Prims.Pure t_ServerDB Prims.l_True (fun _ -> Prims.l_True)
+
+type t_ServerInfo = {
+  f_cert:Bertie.Tls13utils.t_Bytes;
+  f_sk:Bertie.Tls13utils.t_Bytes;
+  f_psk_opt:Core.Option.t_Option Bertie.Tls13utils.t_Bytes
+}
+
+val lookup_db
+      (ciphersuite: Bertie.Tls13crypto.t_Algorithms)
+      (db: t_ServerDB)
+      (sni: Bertie.Tls13utils.t_Bytes)
+      (tkt: Core.Option.t_Option Bertie.Tls13utils.t_Bytes)
+    : Prims.Pure (Core.Result.t_Result t_ServerInfo u8) Prims.l_True (fun _ -> Prims.l_True)
